Upd

code/ecdsap256/Hacl.Impl.P256.MontgomeryMultiplication.fst
@@ -30,7 +30,8 @@ inline_for_extraction noextract
 val montgomery_multiplication_round_: #c: curve -> t: widefelem c -> t2: widefelem c -> 
   Stack unit
     (requires fun h -> live h t /\ live h t2 /\ wide_as_nat c h t2 = 0)
-    (ensures fun h0 _ h1 -> modifies (loc t2) h0 h1 /\ wide_as_nat c h1 t2 < getPower2 c * pow2 64 /\
+    (ensures fun h0 _ h1 -> modifies (loc t2) h0 h1 /\ 
+      wide_as_nat c h1 t2 < getPower2 c * pow2 64 /\
       wide_as_nat c h1 t2 = getPrime c * (wide_as_nat c h0 t % pow2 64))
   
 let montgomery_multiplication_round_ #c t t2 =
@@ -113,24 +114,33 @@ let montgomery_multiplication_round_k0 #c t round k0 =
 
 
 
-val montgomery_multiplication_one_round_proof_st: 
-  #c: curve {(getPrime c + 1) % pow2 64 == 0} ->
-  t: nat {t < getPrime c * getPrime c} -> 
-  result: nat {result = (t + (t % pow2 64) * getPrime c) / pow2 64} ->
-  co: nat {co % getPrime c == t % getPrime c} -> 
-  Lemma (
-    result % getPrime c == co * modp_inv2 #c (pow2 64) % getPrime c  /\
-     result < getPrime c * getPrime c)
-
-
 val lemma_add_lt: a : int -> b: int -> q: int -> q1: int -> Lemma
   (requires (a < q /\ b < q1))
   (ensures (a + b < q + q1))
 
 let lemma_add_lt a b q q1 = ()
 
+val lemma_one_round_0: a: nat -> b1: nat -> b2: nat -> Lemma 
+  (requires (a <= (b1 + pow2 64 * b2) / pow2 64))
+  (ensures (a <= b1 / pow2 64 + b2))
 
-let montgomery_multiplication_one_round_proof_st #c t result co = 
+let lemma_one_round_0 a b1 b2 =
+  lemma_div_plus b1 b2 (pow2 64)
+
+
+
+val montgomery_multiplication_one_round_proof_w_ko: 
+  #c: curve {(getPrime c + 1) % pow2 64 == 0} ->
+  t: nat {t < getPrime c * getPrime c} -> 
+  result: nat {result = (t + (t % pow2 64) * getPrime c) / pow2 64} ->
+  co: nat {co % getPrime c == t % getPrime c} -> 
+  Lemma (
+    result % getPrime c == co * modp_inv2 #c (pow2 64) % getPrime c  /\
+     result < getPrime c * getPrime c /\
+     result <= t / pow2 64 + getPrime c)
+
+
+let montgomery_multiplication_one_round_proof_w_ko #c t result co = 
   let prime = getPrime c in 
   mult_one_round #c t co; 
   mul_lemma_1 (t % pow2 64) (pow2 64) prime; 
@@ -138,21 +148,20 @@ let montgomery_multiplication_one_round_proof_st #c t result co =
   lemma_mult_lt_sqr prime prime (getPower2 c);
   lemma_mult_lt_left (pow2 64) prime (getPower2 c);
   lemma_add_lt (prime * prime) (pow2 64 * prime) (getPower2 c * getPower2 c) (pow2 64 * getPower2 c);
-  assert(prime * prime + pow2 64 * prime < getPower2 c * getPower2 c + pow2 64 * getPower2 c);
   assume (pow2 64 < getPower2 c);
   lemma_mult_lt_right (getPower2 c) (pow2 64) (getPower2 c);
-  assert (getPower2 c * getPower2 c + pow2 64 * getPower2 c < 2 * getPower2 c * getPower2 c);
   pow2_plus (getPower c) (getPower c);
   pow2_double_mult (2 * getPower c); 
-  assert (getPower2 c * getPower2 c + pow2 64 * getPower2 c < pow2 (2 * getPower c + 1));
   lemma_div_lt_nat (getPower2 c * getPower2 c + pow2 64 * getPower2 c) (2 * getPower c + 1) 64;
-  assert ((getPower2 c * getPower2 c + pow2 64 * getPower2 c) / pow2 64 < pow2 (2 * getPower c + 1 - 64));
   assume (getPrime c > pow2 (getPower c - 1));
 
   pow2_plus (getPower c - 1) (getPower c - 1);
   lemma_mult_lt_sqr (pow2 (getPower c - 1)) (pow2 (getPower c - 1)) (getPrime c);
-  pow2_lt_compat (2 * getPower c - 2) (2 * getPower c - 63)
+  pow2_lt_compat (2 * getPower c - 2) (2 * getPower c - 63);
 
+  lemma_mult_lt_right prime (t % pow2 64) (pow2 64);
+  lemma_one_round_0 result t prime
+  
 
 
 val lemma_mod_inv: #c: curve ->  t: int -> Lemma (t % getPrime c = t * modp_inv2 #c (pow2 0) % getPrime c)
@@ -205,7 +214,7 @@ let lemma_inv3 a b c = ()
 
 let lemma_inv2 #c a0 a_i a_i1 i = 
   let prime = getPrime c in 
-  montgomery_multiplication_one_round_proof_st #c a_i a_i1 (a0 * modp_inv2 #c (pow2 (i * 64)));
+  montgomery_multiplication_one_round_proof_w_ko #c a_i a_i1 (a0 * modp_inv2 #c (pow2 (i * 64)));
 
 
   lemma_inv3 a0 (modp_inv2 #c (pow2 (i * 64))) (modp_inv2 #c (pow2 64));
@@ -234,14 +243,27 @@ let lemma_inv2 #c a0 a_i a_i1 i =
     modp_inv2 #c (pow2 ((i + 1) * 64));}
 
 
+val montgomery_multiplication_buffer_by_one_w_ko: #c: curve {(getPrime c + 1) % pow2 64 == 0} 
+  -> a: felem c
+  -> result: felem c -> 
+  Stack unit
+    (requires (fun h -> live h a /\ as_nat c h a < getPrime c /\ live h result)) 
+    (ensures (fun h0 _ h1 -> 
+      let prime = getPrime c in 
+      modifies (loc result) h0 h1 /\ 
+      as_nat c h1 result  = (as_nat c h0 a * modp_inv2_prime (getPower2 c) prime) % prime /\
+      as_nat c h1 result = fromDomain_ #c (as_nat c h0 a)))
 
-let montgomery_multiplication_buffer_by_one #c a result = 
+
+let montgomery_multiplication_buffer_by_one_w_ko #c a result = 
   push_frame();
   
+
   let len = getCoordinateLenU64 c in 
   let t = create (size 2 *! len) (u64 0) in 
     let t_low = sub t (size 0) len in 
     let t_high = sub t len len in 
+
 
   let h0 = ST.get() in 
 
@@ -252,59 +274,295 @@ let montgomery_multiplication_buffer_by_one #c a result =
   let inv h (i: nat { i <= uint_v (getCoordinateLenU64 c)}) = 
     let prime = getPrime c in 
     live h t /\ wide_as_nat c h t < prime * prime  /\
+    modifies (loc t) h0 h /\ 
     wide_as_nat c h t % prime = wide_as_nat c h1 t * modp_inv2 #c (pow2 (i * 64)) % prime
   in 
 
-  assert(wide_as_nat c h0 t = as_nat c h0 t_low + as_nat c h0 t_high * pow2 (v (getCoordinateLenU64 c) * 64));
-  
+  assert(wide_as_nat c h1 t = as_nat c h0 a + as_nat c h0 t_high * getPower2 c);
+  assert(as_nat c h0 t_high = 0);
+
   lemma_inv1 (wide_as_nat c h1 t) (getPrime c);
   lemma_mod_inv #c (wide_as_nat c h1 t);
-  
+
+  let h3 = ST.get() in 
   for 0ul len inv (fun i ->
     let h0_ = ST.get() in 
     montgomery_multiplication_round #c t t; 
     let h1_ = ST.get() in
-    montgomery_multiplication_one_round_proof_st #c (wide_as_nat c h0_ t) (wide_as_nat c h1_ t) (wide_as_nat c h0_ t);
+    montgomery_multiplication_one_round_proof_w_ko #c (wide_as_nat c h0_ t) (wide_as_nat c h1_ t) (wide_as_nat c h0_ t);
     lemma_inv2 #c (wide_as_nat c h1 t) (wide_as_nat c h0_ t) (wide_as_nat c h1_ t) (v i)
   );
 
+
   let h2 = ST.get() in 
-
-  assert (inv h2 (uint_v len));
-  assert (wide_as_nat c h2 t % getPrime c =  wide_as_nat c h1 t * modp_inv2 #c (pow2 ((uint_v len) * 64)) % getPrime c);
-
   
   assume (wide_as_nat c h2 t < 2 * getPrime c);
-  
+
   reduction_prime_2prime_with_carry t result;
-
-  let h3 = ST.get() in 
+  pop_frame();
   
-  assume (as_nat c h3 result = wide_as_nat c h1 t * modp_inv2 #c (pow2 ((uint_v len) * 64)) % getPrime c);
+  lemmaFromDomain #c (as_nat c h0 a)
+
+
+val montgomery_multiplication_buffer_by_one_ko: #c: curve  
+  -> a: felem c
+  -> result: felem c -> 
+  Stack unit
+    (requires (fun h -> live h a /\ as_nat c h a < getPrime c /\ live h result)) 
+    (ensures (fun h0 _ h1 -> 
+      let prime = getPrime c in 
+      modifies (loc result) h0 h1 /\ 
+      as_nat c h1 result  = (as_nat c h0 a * modp_inv2_prime (getPower2 c) prime) % prime /\
+      as_nat c h1 result = fromDomain_ #c (as_nat c h0 a)))
+
+
+let montgomery_multiplication_buffer_by_one_ko #c a result = 
+  push_frame();
+  
+
+  let len = getCoordinateLenU64 c in 
+  let t = create (size 2 *! len) (u64 0) in 
+    let t_low = sub t (size 0) len in 
+    let t_high = sub t len len in 
+
+
+  let h0 = ST.get() in 
+
+  copy t_low a; 
+
+  let h1 = ST.get() in 
+  
+  let inv h (i: nat { i <= uint_v (getCoordinateLenU64 c)}) = 
+    let prime = getPrime c in 
+    live h t /\ wide_as_nat c h t < prime * prime  /\
+    modifies (loc t) h0 h /\ 
+    wide_as_nat c h t % prime = wide_as_nat c h1 t * modp_inv2 #c (pow2 (i * 64)) % prime
+  in 
+
+  assert(wide_as_nat c h1 t = as_nat c h0 a + as_nat c h0 t_high * getPower2 c);
+  assert(as_nat c h0 t_high = 0);
+
+  lemma_inv1 (wide_as_nat c h1 t) (getPrime c);
+  lemma_mod_inv #c (wide_as_nat c h1 t);
+
   admit();
+  let h3 = ST.get() in 
+  for 0ul len inv (fun i ->
+    let h0_ = ST.get() in 
+    montgomery_multiplication_round_k0 #c t t (getKo c); 
+    let h1_ = ST.get() in
+    (* montgomery_multiplication_one_round_proof_w_ko #c (wide_as_nat c h0_ t) (wide_as_nat c h1_ t) (wide_as_nat c h0_ t); *)
+    lemma_inv2 #c (wide_as_nat c h1 t) (wide_as_nat c h0_ t) (wide_as_nat c h1_ t) (v i)
+  );
+
+
+  let h2 = ST.get() in 
   
-  pop_frame()  
+  assume (wide_as_nat c h2 t < 2 * getPrime c);
+
+  reduction_prime_2prime_with_carry t result;
+  pop_frame();
+  
+  lemmaFromDomain #c (as_nat c h0 a)
+
+
+let montgomery_multiplication_buffer_by_one #c a result = 
+  match c with 
+  |P256 -> 
+    assume ((getPrime c + 1) % pow2 64 == 0);
+    montgomery_multiplication_buffer_by_one_w_ko a result
+  |P384 -> montgomery_multiplication_buffer_by_one_ko a result
 
 
 
-let montgomery_multiplication_buffer #c a b result = 
-  assert_norm(prime256 > 3);
+val montgomery_multiplication_buffer_w_k0: #c: curve {(getPrime c + 1) % pow2 64 == 0}
+  -> a: felem c -> b: felem c -> result: felem c ->  
+  Stack unit
+    (requires (fun h ->
+      live h a /\ as_nat c h a < getPrime c /\ live h b /\ live h result /\ as_nat c h b < getPrime c)) 
+    (ensures (fun h0 _ h1 -> 
+      modifies (loc result) h0 h1 /\  
+      as_nat c h1 result < getPrime c /\
+      as_nat c h1 result = (as_nat c h0 a * as_nat c h0 b * modp_inv2_prime (pow2 (getPower c)) (getPrime c)) % getPrime c /\
+      as_nat c h1 result = toDomain_ #c (fromDomain_ #c (as_nat c h0 a) * fromDomain_ #c (as_nat c h0 b) % getPrime c) /\
+      as_nat c h1 result = toDomain_ #c (fromDomain_ #c (as_nat c h0 a) * fromDomain_ #c (as_nat c h0 b))))
+
+
+let montgomery_multiplication_buffer_w_k0 #c a b result = 
   push_frame();
   let len = getCoordinateLenU64 c in 
   
-  let round = create (size 2 *! len) (u64 0) in 
+  let t = create (size 2 *! len) (u64 0) in 
     let h0 = ST.get() in 
-  mul a b round;  
+    
+  mul a b t;  
+
+  let h1 = ST.get() in 
+  
   let inv h (i: nat { i <= uint_v (getCoordinateLenU64 c)}) = 
-    True in 
+    let prime = getPrime c in 
+    live h t /\ wide_as_nat c h t < prime * prime  /\
+    modifies (loc t) h0 h /\ 
+    wide_as_nat c h t % prime = wide_as_nat c h1 t * modp_inv2 #c (pow2 (i * 64)) % prime in
 
-  for 0ul len inv (fun i -> montgomery_multiplication_round #c round round);
-      
-  reduction_prime_2prime_with_carry round result; 
-  pop_frame()  
+  lemma_mult_lt_sqr (as_nat c h0 a) (as_nat c h0 b) (getPrime c);
+  lemma_mod_inv #c (wide_as_nat c h1 t);
+
+  for 0ul len inv (fun i ->
+    let h0_ = ST.get() in
+    montgomery_multiplication_round #c t t; 
+    let h1_ = ST.get() in
+    montgomery_multiplication_one_round_proof_w_ko #c (wide_as_nat c h0_ t) (wide_as_nat c h1_ t) (wide_as_nat c h0_ t);
+    lemma_inv2 #c (wide_as_nat c h1 t) (wide_as_nat c h0_ t) (wide_as_nat c h1_ t) (v i));
+
+  let h2 = ST.get() in 
+  
+  assume (wide_as_nat c h2 t < 2 * getPrime c);
+  reduction_prime_2prime_with_carry t result;
+  
+  pop_frame();
+
+  let prime = getPrime c in 
+  let multResult = as_nat c h0 a * as_nat c h0 b * modp_inv2_prime (pow2 (getPower c)) prime % prime in 
+
+  let a_ = as_nat c h0 a in 
+  let b_ = as_nat c h0 b in 
+  let mod = modp_inv2_prime (pow2 (getPower c)) prime in 
+ 
+  calc (==)
+  {
+    a_ * b_ * mod % prime;
+    (==) {lemmaFromDomainToDomain #c multResult}
+    toDomain_ #c (fromDomain_ #c multResult);
+    (==) {lemmaFromDomain #c multResult}
+    toDomain_ #c ((a_ * b_ * mod  % prime) * mod % prime);
+    (==) {lemma_mod_mul_distr_l (a_ * b_ * mod) mod prime}
+    toDomain_ #c (a_ * b_ * mod * mod % prime);
+    (==) {
+      let open FStar.Tactics in 
+      let open FStar.Tactics.Canon in 
+      assert_by_tactic (a_ * b_ * mod * mod == (a_ * mod) * (b_ * mod)) canon}
+    toDomain_ #c ((a_ * mod) * (b_ * mod) % prime);
+    (==) {
+      lemma_mod_mul_distr_l (a_ * mod) (b_ *  mod) prime; 
+      lemma_mod_mul_distr_r (a_ * mod % prime) (b_ * mod) prime}
+    
+    toDomain_ #c ((a_ * mod % prime) * (b_ * mod % prime) % prime);
+    (==) {lemmaFromDomain #c a_; lemmaFromDomain #c b_}
+    toDomain_ #c (fromDomain_ #c a_ * fromDomain_ #c b_ % prime);
+
+  };
+
+  inDomain_mod_is_not_mod #c (fromDomain_ #c a_ * fromDomain_ #c b_)
 
 
-let montgomery_square_buffer #c a result = 
+
+val montgomery_multiplication_buffer_k0: #c: curve
+  -> a: felem c -> b: felem c -> result: felem c ->  
+  Stack unit
+    (requires (fun h ->
+      live h a /\ as_nat c h a < getPrime c /\ live h b /\ live h result /\ as_nat c h b < getPrime c)) 
+    (ensures (fun h0 _ h1 -> 
+      modifies (loc result) h0 h1 /\  
+      as_nat c h1 result < getPrime c /\
+      as_nat c h1 result = (as_nat c h0 a * as_nat c h0 b * modp_inv2_prime (pow2 (getPower c)) (getPrime c)) % getPrime c /\
+      as_nat c h1 result = toDomain_ #c (fromDomain_ #c (as_nat c h0 a) * fromDomain_ #c (as_nat c h0 b) % getPrime c) /\
+      as_nat c h1 result = toDomain_ #c (fromDomain_ #c (as_nat c h0 a) * fromDomain_ #c (as_nat c h0 b))))
+
+
+let montgomery_multiplication_buffer_k0 #c a b result = 
+  push_frame();
+  let len = getCoordinateLenU64 c in 
+
+  let t = create (size 2 *! len) (u64 0) in 
+    let h0 = ST.get() in 
+    
+  mul a b t;  
+
+  let h1 = ST.get() in 
+  
+  let inv h (i: nat { i <= uint_v (getCoordinateLenU64 c)}) = 
+    let prime = getPrime c in 
+    live h t /\ wide_as_nat c h t < prime * prime  /\
+    modifies (loc t) h0 h /\ 
+    wide_as_nat c h t % prime = wide_as_nat c h1 t * modp_inv2 #c (pow2 (i * 64)) % prime in
+
+  lemma_mult_lt_sqr (as_nat c h0 a) (as_nat c h0 b) (getPrime c);
+  lemma_mod_inv #c (wide_as_nat c h1 t);
+
+  assume (inv h1 0);
+  for 0ul len inv (fun i ->
+    let h0_ = ST.get() in
+    montgomery_multiplication_round_k0 #c t t (getKo c); 
+    let h1_ = ST.get() in
+    admit();
+    montgomery_multiplication_one_round_proof_w_ko #c (wide_as_nat c h0_ t) (wide_as_nat c h1_ t) (wide_as_nat c h0_ t);
+    lemma_inv2 #c (wide_as_nat c h1 t) (wide_as_nat c h0_ t) (wide_as_nat c h1_ t) (v i));
+
+  let h2 = ST.get() in 
+  
+  assume (wide_as_nat c h2 t < 2 * getPrime c);
+  reduction_prime_2prime_with_carry t result;
+  
+  pop_frame();
+
+  let prime = getPrime c in 
+  let multResult = as_nat c h0 a * as_nat c h0 b * modp_inv2_prime (pow2 (getPower c)) prime % prime in 
+
+  let a_ = as_nat c h0 a in 
+  let b_ = as_nat c h0 b in 
+  let mod = modp_inv2_prime (pow2 (getPower c)) prime in 
+
+  admit();
+  calc (==)
+  {
+    a_ * b_ * mod % prime;
+    (==) {lemmaFromDomainToDomain #c multResult}
+    toDomain_ #c (fromDomain_ #c multResult);
+    (==) {lemmaFromDomain #c multResult}
+    toDomain_ #c ((a_ * b_ * mod  % prime) * mod % prime);
+    (==) {lemma_mod_mul_distr_l (a_ * b_ * mod) mod prime}
+    toDomain_ #c (a_ * b_ * mod * mod % prime);
+    (==) {
+      let open FStar.Tactics in 
+      let open FStar.Tactics.Canon in 
+      assert_by_tactic (a_ * b_ * mod * mod == (a_ * mod) * (b_ * mod)) canon}
+    toDomain_ #c ((a_ * mod) * (b_ * mod) % prime);
+    (==) {
+      lemma_mod_mul_distr_l (a_ * mod) (b_ *  mod) prime; 
+      lemma_mod_mul_distr_r (a_ * mod % prime) (b_ * mod) prime}
+    
+    toDomain_ #c ((a_ * mod % prime) * (b_ * mod % prime) % prime);
+    (==) {lemmaFromDomain #c a_; lemmaFromDomain #c b_}
+    toDomain_ #c (fromDomain_ #c a_ * fromDomain_ #c b_ % prime);
+
+  };
+
+  inDomain_mod_is_not_mod #c (fromDomain_ #c a_ * fromDomain_ #c b_)
+
+
+let montgomery_multiplication_buffer #c a b result = 
+  match c with 
+  |P256 ->
+    assume ((getPrime c + 1) % pow2 64 == 0);
+    montgomery_multiplication_buffer_w_k0 a b result
+  |P384 -> montgomery_multiplication_buffer_k0 a b result
+
+
+val montgomery_square_buffer_w_k0: #c: curve {(getPrime c + 1) % pow2 64 == 0} -> a: felem c -> result: felem c ->  
+  Stack unit
+    (requires (fun h -> live h a /\ as_nat c h a < (getPrime c) /\ live h result)) 
+    (ensures (fun h0 _ h1 -> 
+      (
+	let prime = getPrime c in 
+	modifies (loc result) h0 h1 /\  
+	as_nat c h1 result < prime /\ 
+	as_nat c h1 result = (as_nat c h0 a * as_nat c h0 a * modp_inv2_prime (getPower c) prime) % prime /\
+	as_nat c h1 result = toDomain_ #c (fromDomain_ #c (as_nat c h0 a) * fromDomain_ #c (as_nat c h0 a) % prime) /\
+	as_nat c h1 result = toDomain_ #c (fromDomain_ #c (as_nat c h0 a) * fromDomain_ #c (as_nat c h0 a)))))
+
+
+let montgomery_square_buffer_w_k0 #c a result = 
   assert_norm(prime256 > 3);
   push_frame();
     
@@ -313,13 +571,52 @@ let montgomery_square_buffer #c a result =
     let h0 = ST.get() in 
   square_bn a t;  
     let h1 = ST.get() in 
-    mul_lemma_ (as_nat P256 h0 a) (as_nat P256 h0 a) prime256;
+    (* mul_lemma_ (as_nat c h0 a) (as_nat P256 h0 a) prime256; *)
 
-  let len = getCoordinateLenU64 c in 
-  let inv h (i: nat { i <= uint_v (getCoordinateLenU64 c)}) = True in 
-  for 0ul len inv (fun i -> montgomery_multiplication_round #c t t);
+  let inv h (i: nat { i <= uint_v len}) = True in 
+    for 0ul len inv (fun i ->  montgomery_multiplication_round #c t t);
 
   reduction_prime_2prime_with_carry t result; 
+  admit();
    
   pop_frame()  
 
+
+
+val montgomery_square_buffer_k0: #c: curve -> a: felem c -> result: felem c ->  
+  Stack unit
+    (requires (fun h -> live h a /\ as_nat c h a < (getPrime c) /\ live h result)) 
+    (ensures (fun h0 _ h1 -> 
+      (
+	let prime = getPrime c in 
+	modifies (loc result) h0 h1 /\  
+	as_nat c h1 result < prime /\ 
+	as_nat c h1 result = (as_nat c h0 a * as_nat c h0 a * modp_inv2_prime (getPower c) prime) % prime /\
+	as_nat c h1 result = toDomain_ #c (fromDomain_ #c (as_nat c h0 a) * fromDomain_ #c (as_nat c h0 a) % prime) /\
+	as_nat c h1 result = toDomain_ #c (fromDomain_ #c (as_nat c h0 a) * fromDomain_ #c (as_nat c h0 a)))))
+
+
+let montgomery_square_buffer_k0 #c a result = 
+  assert_norm(prime256 > 3);
+  push_frame();
+    
+  let len = getCoordinateLenU64 c in 
+  let t = create (size 2 *! len) (u64 0) in 
+    let h0 = ST.get() in 
+  square_bn a t;  
+    let h1 = ST.get() in 
+    (* mul_lemma_ (as_nat c h0 a) (as_nat P256 h0 a) prime256; *)
+
+  let inv h (i: nat { i <= uint_v len}) = True in 
+    for 0ul len inv (fun i ->  montgomery_multiplication_round_k0 #c t t (getKo c) );
+
+  reduction_prime_2prime_with_carry t result; 
+  admit();
+   
+  pop_frame()  
+
+
+let montgomery_square_buffer #c a result = 
+  match c with 
+  |P256 -> montgomery_square_buffer_w_k0 a result
+  |P384 -> montgomery_square_buffer_k0 a result
