code/ecdsap256/Hacl.Impl.SolinasReduction.P384.fst
@@ -1,0 +1,767 @@
+module Hacl.Impl.SolinasReduction.P384
+
+open FStar.HyperStack.All
+open FStar.HyperStack
+module ST = FStar.HyperStack.ST
+
+open Lib.IntTypes
+open FStar.Math.Lemmas
+open FStar.Math.Lib
+open Lib.Buffer
+
+open Spec.P256
+open Hacl.Spec.P256.Definition
+open Hacl.Impl.P.LowLevel
+
+open FStar.Mul
+
+module BV = FStar.BitVector
+module Seq = FStar.Seq
+
+
+#set-options "--fuel 0 --ifuel 0 --z3rlimit 50"
+(* http://citeseerx.ist.psu.edu/viewdoc/download?doi=10.1.1.46.2133&rep=rep1&type=pdf *)
+
+inline_for_extraction noextract
+val get_high_part: a:uint64 -> r:uint32{uint_v r == uint_v a / pow2 32}
+let get_high_part a = to_u32 (shift_right a (size 32))
+
+inline_for_extraction noextract
+val get_low_part: a:uint64 -> r:uint32{uint_v r == uint_v a % pow2 32}
+let get_low_part a = to_u32 a
+
+(* ^^ *)
+
+val shift_bound: #n:nat -> num:UInt.uint_t n -> n':nat ->
+  Lemma (num * pow2 n' <= pow2 (n' + n) - pow2 n')
+
+let shift_bound #n num n' =
+  Math.Lemmas.lemma_mult_le_right (pow2 n') num (pow2 n - 1);
+  Math.Lemmas.distributivity_sub_left (pow2 n) 1 (pow2 n');
+  Math.Lemmas.pow2_plus n' n
+
+
+val logxor_vec_append (#n1 #n2: pos) (a1 b1: BV.bv_t n1) (a2 b2: BV.bv_t n2) :
+  Lemma (Seq.append (BV.logxor_vec a1 b1) (BV.logxor_vec a2 b2) ==
+         BV.logxor_vec #(n1 + n2) (FStar.Seq.append a1 a2) (FStar.Seq.append b1 b2))
+
+let logxor_vec_append #n1 #n2 a1 b1 a2 b2 =
+  Seq.lemma_eq_intro (Seq.append (BV.logxor_vec a1 b1) (BV.logxor_vec a2 b2))
+                     (BV.logxor_vec #(n1 + n2) (Seq.append a1 a2) (Seq.append b1 b2))
+
+val append_uint: #n1:nat -> #n2:nat
+  -> num1:UInt.uint_t n1 -> num2:UInt.uint_t n2 -> UInt.uint_t (n1 + n2)
+
+let append_uint #n1 #n2 num1 num2 =
+  shift_bound num2 n1;
+  num1 + num2 * pow2 n1
+
+val to_vec_append : #n1:pos-> #n2:pos -> num1:UInt.uint_t n1 -> num2:UInt.uint_t n2 ->
+  Lemma (UInt.to_vec (append_uint num1 num2) ==
+         Seq.append (UInt.to_vec num2) (UInt.to_vec num1))
+
+let to_vec_append #n1 #n2 num1 num2 =
+  UInt.append_lemma (UInt.to_vec num2) (UInt.to_vec num1)
+
+val to_vec_low_high: a:UInt.uint_t 64 -> Lemma
+  (UInt.to_vec a ==
+   Seq.append (UInt.to_vec #32 (a / pow2 32)) (UInt.to_vec #32 (a % pow2 32)))
+
+let to_vec_low_high a =
+  assert (a == append_uint #32 #32 (a % pow2 32) (a / pow2 32));
+  to_vec_append #32 #32 (a % pow2 32) (a / pow2 32)
+
+
+val lemma_xor_zero:
+    low:  uint64{v (get_high_part low) == 0}
+  -> high: uint64{v (get_low_part high) == 0}
+  -> Lemma (v (logxor low high) = v high + v low)
+
+let lemma_xor_zero l h =
+  to_vec_low_high (v h);
+  to_vec_low_high (v l);
+  let a1 = BV.zero_vec #32 in
+  let a2 = UInt.to_vec #32 (v l % pow2 32) in
+  let b1 = UInt.to_vec #32 (v h / pow2 32) in
+  let b2 = BV.zero_vec #32 in
+  assert (Seq.equal (UInt.to_vec (UInt.zero 32)) (BV.zero_vec #32));
+  assert (UInt.to_vec #64 (UInt.logxor (v l) (v h)) ==
+          BV.logxor_vec (Seq.append a1 a2) (Seq.append b1 b2));
+  logxor_vec_append a1 b1 a2 b2;
+  assert (Seq.equal (BV.logxor_vec a1 b1) b1);
+  assert (Seq.equal (BV.logxor_vec a2 b2) a2);
+  UInt.append_lemma b1 a2;
+  logxor_spec l h
+
+
+val store_high_low_u: high:uint32 -> low:uint32 -> r:uint64{v r = v high * pow2 32 + v low}
+
+let store_high_low_u high low =
+  let as_uint64_high = to_u64 high in
+  let as_uint64_high = Lib.IntTypes.shift_left as_uint64_high (size 32) in
+  let as_uint64_low = to_u64 low in
+  assert (v as_uint64_high = v high * pow2 32);
+  assert (v as_uint64_low = v low);
+  lemma_xor_zero as_uint64_low as_uint64_high;
+  logxor as_uint64_low as_uint64_high
+
+
+(* / ^^ *)
+
+
+inline_for_extraction noextract
+val load_buffer: a0: uint64 -> a1: uint64 -> a2: uint64 -> a3: uint64 -> a4: uint64 -> a5: uint64
+  -> o: lbuffer uint64 (size 6)
+  -> Stack unit
+  (requires fun h -> live h o)
+  (ensures  fun h0 _ h1 -> modifies (loc o) h0 h1 /\
+    as_nat P384 h1 o = v a0  + v a1 * pow2 (2 * 32) + v a2 * pow2 (4 * 32)  + v a3 * pow2 (6 * 32) + v a4 * pow2 (8 * 32) + v a5 * pow2 (10 * 32))
+
+
+let load_buffer a0 a1 a2 a3 a4 a5 o =
+  assert(pow2 (2 * 32) = pow2 64);
+  assert(pow2 (4 * 32) = pow2 (2 * 64));
+  assert(pow2 (6 * 32) = pow2 (3 * 64));
+  assert(pow2 (8 * 32) = pow2 (4 * 64));
+  assert(pow2 (10 * 32) = pow2 (5 * 64));  
+  
+  upd o (size 0) a0;
+  upd o (size 1) a1;
+  upd o (size 2) a2;
+  upd o (size 3) a3;
+  upd o (size 4) a4;
+  upd o (size 5) a5
+
+
+val upl_zer_buffer: c0: uint32 -> c1: uint32 ->  c2: uint32 ->  c3: uint32 ->  
+  c4: uint32 ->  c5: uint32 ->  c6: uint32 ->  c7: uint32 ->  c8: uint32 ->  c9: uint32 ->  
+  c10: uint32 ->  c11: uint32 -> o: lbuffer uint64 (size 6) -> 
+  Stack unit 
+    (requires fun h -> live h o)
+    (ensures fun h0 _ h1 -> modifies (loc o) h0 h1 /\ 
+      as_nat P384 h1 o == (v c0 + v c1 * pow2 (1 * 32) + v c2 * pow2 (2 * 32) + v c3 * pow2 (3 * 32) + v c4 * pow2 (4 * 32) + v c5 * pow2 (5 * 32) + v c6 * pow2 (6 * 32) + v c7 * pow2 (7 * 32) + v c8 * pow2 (8 * 32) + v c9 * pow2 (9 * 32) + v c10 * pow2 (10 * 32) + v c11 * pow2 (11 * 32)) % prime384)
+
+
+let upl_zer_buffer c0 c1 c2 c3 c4 c5 c6 c7 c8 c9 c10 c11 o = 
+  assert_norm (pow2 (1 * 32) * pow2 (2 * 32) = pow2 (3 * 32));
+  assert_norm (pow2 (2 * 32) * pow2 (2 * 32) = pow2 (4 * 32));
+  assert_norm (pow2 (3 * 32) * pow2 (2 * 32) = pow2 (5 * 32));
+  assert_norm (pow2 (4 * 32) * pow2 (2 * 32) = pow2 (6 * 32));
+  assert_norm (pow2 (5 * 32) * pow2 (2 * 32) = pow2 (7 * 32));
+  assert_norm (pow2 (6 * 32) * pow2 (2 * 32) = pow2 (8 * 32));
+  assert_norm (pow2 (7 * 32) * pow2 (2 * 32) = pow2 (9 * 32));
+  assert_norm (pow2 (8 * 32) * pow2 (2 * 32) = pow2 (10 * 32));
+  assert_norm (pow2 (9 * 32) * pow2 (2 * 32) = pow2 (11 * 32));
+
+  let b0 = store_high_low_u c1 c0 in 
+  let b1 = store_high_low_u c3 c2 in 
+  let b2 = store_high_low_u c5 c4 in 
+  let b3 = store_high_low_u c7 c6 in 
+  let b4 = store_high_low_u c9 c8 in 
+  let b5 = store_high_low_u c11 c10 in 
+
+  load_buffer b0 b1 b2 b3 b4 b5 o;
+  reduction_prime_2prime #P384 o o
+
+
+val upl_fir_buffer: c21: uint32 -> c22: uint32 -> c23: uint32 -> o: lbuffer uint64 (size 6) -> 
+  Stack unit 
+    (requires fun h -> live h o)
+    (ensures fun h0 _ h1 -> modifies (loc o) h0 h1 /\
+      as_nat P384 h1 o == (v c21 * pow2 (4 * 32) + v c22 * pow2 (5 * 32) + v c23 * pow2 (6 * 32)) % prime384)
+
+let upl_fir_buffer c21 c22 c23 o = 
+  assert_norm (pow2 (1 * 32) * pow2 (2 * 32) = pow2 (3 * 32));
+  assert_norm (pow2 (2 * 32) * pow2 (2 * 32) = pow2 (4 * 32));  assert_norm (pow2 (3 * 32) * pow2 (2 * 32) = pow2 (5 * 32));
+  assert_norm (pow2 (4 * 32) * pow2 (2 * 32) = pow2 (6 * 32));
+  assert_norm (pow2 (5 * 32) * pow2 (2 * 32) = pow2 (7 * 32));
+
+  let b0 = store_high_low_u (u32 0) (u32 0) in 
+  let b1 = store_high_low_u (u32 0) (u32 0) in 
+  let b2 = store_high_low_u c22 c21 in 
+  let b3 = store_high_low_u (u32 0) c23 in 
+  let b4 = store_high_low_u (u32 0) (u32 0) in 
+  let b5 = store_high_low_u (u32 0) (u32 0) in 
+
+  load_buffer b0 b1 b2 b3 b4 b5 o;
+    let h1 = ST.get() in 
+    assert_norm (pow2 (7 * 32) < prime384);
+  modulo_lemma (as_nat P384 h1 o) prime384
+
+
+val upl_sec_buffer: c12: uint32 -> c13: uint32 -> c14: uint32 -> c15: uint32 -> c16: uint32 -> c17: uint32 -> c18: uint32 -> c19: uint32 -> c20: uint32 -> c21: uint32 -> c22: uint32 -> c23: uint32 -> 
+o: lbuffer uint64 (size 6) -> 
+  Stack unit
+    (requires fun h -> live h o)
+    (ensures fun h0 _ h1 -> modifies (loc o) h0 h1 /\
+      as_nat P384 h1 o == (v c12 + v c13 * pow2 (1 * 32) + v c14 * pow2 (2 * 32) + v c15 * pow2 (3 * 32) + v c16 * pow2 (4 * 32) + v c17 * pow2 (5 * 32) + v c18 * pow2 (6 * 32) + v c19 * pow2 (7 * 32) + v c20 * pow2 (8 * 32) + v c21 * pow2 (9 * 32) + v c22 * pow2 (10 * 32) + v c23 * pow2 (11 * 32)) % prime384)
+
+let upl_sec_buffer c12 c13 c14 c15 c16 c17 c18 c19 c20 c21 c22 c23 o = 
+  assert_norm (pow2 (1 * 32) * pow2 (2 * 32) = pow2 (3 * 32));
+  assert_norm (pow2 (2 * 32) * pow2 (2 * 32) = pow2 (4 * 32));
+  assert_norm (pow2 (3 * 32) * pow2 (2 * 32) = pow2 (5 * 32));
+  assert_norm (pow2 (4 * 32) * pow2 (2 * 32) = pow2 (6 * 32));
+  assert_norm (pow2 (5 * 32) * pow2 (2 * 32) = pow2 (7 * 32));
+  assert_norm (pow2 (6 * 32) * pow2 (2 * 32) = pow2 (8 * 32));
+  assert_norm (pow2 (7 * 32) * pow2 (2 * 32) = pow2 (9 * 32));
+  assert_norm (pow2 (8 * 32) * pow2 (2 * 32) = pow2 (10 * 32));
+  assert_norm (pow2 (9 * 32) * pow2 (2 * 32) = pow2 (11 * 32));
+
+  let b0 = store_high_low_u c13 c12 in 
+  let b1 = store_high_low_u c15 c14 in 
+  let b2 = store_high_low_u c17 c16 in 
+  let b3 = store_high_low_u c19 c18 in 
+  let b4 = store_high_low_u c21 c20 in 
+  let b5 = store_high_low_u c23 c22 in 
+
+  load_buffer b0 b1 b2 b3 b4 b5 o;
+  reduction_prime_2prime #P384 o o
+
+
+val upl_thi_buffer: c12: uint32 -> c13: uint32 -> c14: uint32 -> c15: uint32 -> c16: uint32 -> c17: uint32 -> c18: uint32 -> c19: uint32 -> c20: uint32 -> c21: uint32 -> c22: uint32 -> c23: uint32 -> o: lbuffer uint64 (size 6) -> 
+  Stack unit 
+    (requires fun h -> live h o)
+    (ensures fun h0 _ h1 -> modifies (loc o) h0 h1 /\ 
+      as_nat P384 h1 o = (v c21 + v c22 * pow2 (1 * 32) + v c23 * pow2 (2 * 32) + v c12 * pow2 (3 * 32) + v c13 * pow2 (4 * 32) + v c14 * pow2 (5 * 32) + v c15 * pow2 (6 * 32) + v c16 * pow2 (7 * 32) + v c17 * pow2 (8 * 32) + v c18 * pow2 (9 * 32) + v c19 * pow2 (10 * 32) + v c20 * pow2 (11 * 32)) % prime384)
+    
+
+let upl_thi_buffer c12 c13 c14 c15 c16 c17 c18 c19 c20 c21 c22 c23 o = 
+  assert_norm (pow2 (1 * 32) * pow2 (2 * 32) = pow2 (3 * 32));
+  assert_norm (pow2 (2 * 32) * pow2 (2 * 32) = pow2 (4 * 32));
+  assert_norm (pow2 (3 * 32) * pow2 (2 * 32) = pow2 (5 * 32));
+  assert_norm (pow2 (4 * 32) * pow2 (2 * 32) = pow2 (6 * 32));
+  assert_norm (pow2 (5 * 32) * pow2 (2 * 32) = pow2 (7 * 32));
+  assert_norm (pow2 (6 * 32) * pow2 (2 * 32) = pow2 (8 * 32));
+  assert_norm (pow2 (7 * 32) * pow2 (2 * 32) = pow2 (9 * 32));
+  assert_norm (pow2 (8 * 32) * pow2 (2 * 32) = pow2 (10 * 32));
+  assert_norm (pow2 (9 * 32) * pow2 (2 * 32) = pow2 (11 * 32));
+
+  let b0 = store_high_low_u c22 c21 in 
+  let b1 = store_high_low_u c12 c23 in 
+  let b2 = store_high_low_u c14 c13 in 
+  let b3 = store_high_low_u c16 c15 in 
+  let b4 = store_high_low_u c18 c17 in 
+  let b5 = store_high_low_u c20 c19 in 
+
+  load_buffer b0 b1 b2 b3 b4 b5 o;
+  reduction_prime_2prime #P384 o o    
+
+
+val upl_forth_buffer: c12: uint32 -> c13: uint32 -> c14: uint32 -> c15: uint32 -> c16: uint32 -> c17: uint32 -> c18: uint32 -> c19: uint32-> c20: uint32 -> c23: uint32 -> 
+o: lbuffer uint64 (size 6) -> 
+  Stack unit 
+    (requires fun h -> live h o) 
+    (ensures fun h0 _ h1 -> modifies (loc o) h0 h1 /\ 
+      as_nat P384 h1 o = (v c23 * pow2 (1 * 32) + v c20 * pow2 (3 * 32) + v c12 * pow2 (4 * 32) + v c13 * pow2 (5 * 32) + v c14 * pow2 (6 * 32) + v c15 * pow2 (7 * 32) + v c16 * pow2 (8 * 32) + v c17 * pow2 (9 * 32) + v c18 * pow2 (10 * 32) + v c19 * pow2 (11 * 32)) % prime384)
+
+
+let upl_forth_buffer c12 c13 c14 c15 c16 c17 c18 c19 c20 c23 o = 
+  assert_norm (pow2 (1 * 32) * pow2 (2 * 32) = pow2 (3 * 32));
+  assert_norm (pow2 (2 * 32) * pow2 (2 * 32) = pow2 (4 * 32));
+  assert_norm (pow2 (3 * 32) * pow2 (2 * 32) = pow2 (5 * 32));
+  assert_norm (pow2 (4 * 32) * pow2 (2 * 32) = pow2 (6 * 32));
+  assert_norm (pow2 (5 * 32) * pow2 (2 * 32) = pow2 (7 * 32));
+  assert_norm (pow2 (6 * 32) * pow2 (2 * 32) = pow2 (8 * 32));
+  assert_norm (pow2 (7 * 32) * pow2 (2 * 32) = pow2 (9 * 32));
+  assert_norm (pow2 (8 * 32) * pow2 (2 * 32) = pow2 (10 * 32));
+  assert_norm (pow2 (9 * 32) * pow2 (2 * 32) = pow2 (11 * 32));
+
+  let b0 = store_high_low_u c23 (u32 0) in 
+  let b1 = store_high_low_u c20 (u32 0) in 
+  let b2 = store_high_low_u c13 c12 in 
+  let b3 = store_high_low_u c15 c14 in 
+  let b4 = store_high_low_u c17 c16 in 
+  let b5 = store_high_low_u c19 c18 in 
+
+  load_buffer b0 b1 b2 b3 b4 b5 o;
+  reduction_prime_2prime #P384 o o
+
+
+val upl_fif_buffer: c20: uint32 -> c21: uint32 -> c22: uint32 -> c23: uint32 -> 
+  o: lbuffer uint64 (size 6) -> 
+  Stack unit 
+    (requires fun h -> live h o)
+    (ensures fun h0 _ h1 -> modifies (loc o) h0 h1 /\
+      as_nat P384 h1 o = ((v c20 * pow2 (4 * 32) + v c21 * pow2 (5 * 32) + v c22 * pow2 (6 * 32) + v c23 * pow2 (7 * 32)) % prime384))
+     
+let upl_fif_buffer c20 c21 c22 c23 o = 
+  assert_norm (pow2 (1 * 32) * pow2 (2 * 32) = pow2 (3 * 32));
+  assert_norm (pow2 (2 * 32) * pow2 (2 * 32) = pow2 (4 * 32));
+  assert_norm (pow2 (3 * 32) * pow2 (2 * 32) = pow2 (5 * 32));
+  assert_norm (pow2 (4 * 32) * pow2 (2 * 32) = pow2 (6 * 32));
+  assert_norm (pow2 (5 * 32) * pow2 (2 * 32) = pow2 (7 * 32));
+  assert_norm (pow2 (6 * 32) * pow2 (2 * 32) = pow2 (8 * 32));
+  assert_norm (pow2 (7 * 32) * pow2 (2 * 32) = pow2 (9 * 32));
+  assert_norm (pow2 (8 * 32) * pow2 (2 * 32) = pow2 (10 * 32));
+  assert_norm (pow2 (9 * 32) * pow2 (2 * 32) = pow2 (11 * 32));
+
+  let b0 = store_high_low_u (u32 0) (u32 0) in 
+  let b1 = store_high_low_u (u32 0) (u32 0) in 
+  let b2 = store_high_low_u c21 c20 in 
+  let b3 = store_high_low_u c23 c22 in 
+  let b4 = store_high_low_u (u32 0) (u32 0) in 
+  let b5 = store_high_low_u (u32 0) (u32 0) in 
+
+  load_buffer b0 b1 b2 b3 b4 b5 o;
+  reduction_prime_2prime #P384 o o;
+      let h1 = ST.get() in 
+  assert_norm (pow2 (8 * 32) < prime384);
+  modulo_lemma (as_nat P384 h1 o) prime384
+
+
+val upl_six_buffer: c20: uint32 -> c21: uint32 -> c22: uint32 -> c23: uint32 -> 
+  o: lbuffer uint64 (size 6) -> 
+  Stack unit 
+    (requires fun h -> live h o)
+    (ensures fun h0 _ h1 -> modifies (loc o) h0 h1 /\
+      as_nat P384 h1 o == (v c20 + v c21 * pow2 (3 * 32) + v c22 * pow2 (4 * 32) + v c23 * pow2 (5 * 32)) % prime384)
+
+let upl_six_buffer c20 c21 c22 c23 o =
+  assert_norm (pow2 (1 * 32) * pow2 (2 * 32) = pow2 (3 * 32));
+  assert_norm (pow2 (2 * 32) * pow2 (2 * 32) = pow2 (4 * 32));
+  assert_norm (pow2 (3 * 32) * pow2 (2 * 32) = pow2 (5 * 32));
+  assert_norm (pow2 (4 * 32) * pow2 (2 * 32) = pow2 (6 * 32));
+  assert_norm (pow2 (5 * 32) * pow2 (2 * 32) = pow2 (7 * 32));
+  assert_norm (pow2 (6 * 32) * pow2 (2 * 32) = pow2 (8 * 32));
+  assert_norm (pow2 (7 * 32) * pow2 (2 * 32) = pow2 (9 * 32));
+  assert_norm (pow2 (8 * 32) * pow2 (2 * 32) = pow2 (10 * 32));
+  assert_norm (pow2 (9 * 32) * pow2 (2 * 32) = pow2 (11 * 32));
+
+  let b0 = store_high_low_u (u32 0) c20 in 
+  let b1 = store_high_low_u c21 (u32 0) in 
+  let b2 = store_high_low_u c23 c22 in 
+  let b3 = store_high_low_u (u32 0) (u32 0) in 
+  let b4 = store_high_low_u (u32 0) (u32 0) in 
+  let b5 = store_high_low_u (u32 0) (u32 0) in 
+
+  load_buffer b0 b1 b2 b3 b4 b5 o;
+  reduction_prime_2prime #P384 o o;
+      let h1 = ST.get() in 
+  assert_norm (pow2 (6 * 32) < prime384);
+  modulo_lemma (as_nat P384 h1 o) prime384
+
+
+val upl_sev_buffer: c12: uint32 -> c13: uint32 -> c14: uint32 -> c15: uint32 -> c16: uint32 -> c17: uint32 -> c18: uint32 -> c19: uint32 -> c20: uint32 -> c21: uint32 -> c22: uint32 -> c23: uint32 -> 
+  o: lbuffer uint64 (size 6) ->
+  Stack unit 
+    (requires fun h -> live h o)
+    (ensures fun h0 _ h1 -> modifies (loc o) h0 h1 /\ 
+    as_nat P384 h1 o = (v c23 + v c12 * pow2 (1 * 32) + v c13 * pow2 (2 * 32) + v c14 * pow2 (3 * 32) + v c15 * pow2 (4 * 32) + v c16 * pow2 (5 * 32) + v c17 * pow2 (6 * 32) + v c18 * pow2 (7 * 32) + v c19 * pow2 (8 * 32) + v c20 * pow2 (9 * 32) + v c21 * pow2 (10 * 32) + v c22 * pow2 (11 * 32)) % prime384)
+      
+let upl_sev_buffer c12 c13 c14 c15 c16 c17 c18 c19 c20 c21 c22 c23 o = 
+  assert_norm (pow2 (1 * 32) * pow2 (2 * 32) = pow2 (3 * 32));
+  assert_norm (pow2 (2 * 32) * pow2 (2 * 32) = pow2 (4 * 32));
+  assert_norm (pow2 (3 * 32) * pow2 (2 * 32) = pow2 (5 * 32));
+  assert_norm (pow2 (4 * 32) * pow2 (2 * 32) = pow2 (6 * 32));
+  assert_norm (pow2 (5 * 32) * pow2 (2 * 32) = pow2 (7 * 32));
+  assert_norm (pow2 (6 * 32) * pow2 (2 * 32) = pow2 (8 * 32));
+  assert_norm (pow2 (7 * 32) * pow2 (2 * 32) = pow2 (9 * 32));
+  assert_norm (pow2 (8 * 32) * pow2 (2 * 32) = pow2 (10 * 32));
+  assert_norm (pow2 (9 * 32) * pow2 (2 * 32) = pow2 (11 * 32));
+
+  let b0 = store_high_low_u c12 c23 in 
+  let b1 = store_high_low_u c14 c13 in 
+  let b2 = store_high_low_u c16 c15 in 
+  let b3 = store_high_low_u c18 c17 in 
+  let b4 = store_high_low_u c20 c19 in 
+  let b5 = store_high_low_u c22 c21 in 
+
+  load_buffer b0 b1 b2 b3 b4 b5 o;
+  reduction_prime_2prime #P384 o o
+
+
+val upl_eit_buffer: c20: uint32 -> c21: uint32 -> c22: uint32 -> c23: uint32 -> 
+  o: lbuffer uint64 (size 6) ->
+  Stack unit 
+    (requires fun h -> live h o)
+    (ensures fun h0 _ h1 -> modifies (loc o) h0 h1 /\
+      as_nat P384 h1 o = (v c20 * pow2 (1 * 32) + v c21 * pow2 (2 * 32) + v c22 * pow2 (3 * 32) + v c23 * pow2 (4 * 32)) % prime384)
+
+let upl_eit_buffer c20 c21 c22 c23 o = 
+  assert_norm (pow2 (1 * 32) * pow2 (2 * 32) = pow2 (3 * 32));
+  assert_norm (pow2 (2 * 32) * pow2 (2 * 32) = pow2 (4 * 32));
+  assert_norm (pow2 (3 * 32) * pow2 (2 * 32) = pow2 (5 * 32));
+  assert_norm (pow2 (4 * 32) * pow2 (2 * 32) = pow2 (6 * 32));
+  assert_norm (pow2 (5 * 32) * pow2 (2 * 32) = pow2 (7 * 32));
+  assert_norm (pow2 (6 * 32) * pow2 (2 * 32) = pow2 (8 * 32));
+  assert_norm (pow2 (7 * 32) * pow2 (2 * 32) = pow2 (9 * 32));
+  assert_norm (pow2 (8 * 32) * pow2 (2 * 32) = pow2 (10 * 32));
+  assert_norm (pow2 (9 * 32) * pow2 (2 * 32) = pow2 (11 * 32));
+
+  let b0 = store_high_low_u c20 (u32 0) in 
+  let b1 = store_high_low_u c22 c21 in 
+  let b2 = store_high_low_u (u32 0) c23 in 
+  let b3 = store_high_low_u (u32 0) (u32 0) in 
+  let b4 = store_high_low_u (u32 0) (u32 0) in 
+  let b5 = store_high_low_u (u32 0) (u32 0) in 
+
+  load_buffer b0 b1 b2 b3 b4 b5 o;
+  reduction_prime_2prime #P384 o o;
+      let h1 = ST.get() in 
+  assert_norm (pow2 (6 * 32) < prime384);
+  modulo_lemma (as_nat P384 h1 o) prime384
+
+
+val upl_nin_buffer: c23: uint32 -> 
+  o: lbuffer uint64 (size 6) -> 
+  Stack unit 
+    (requires fun h -> live h o)
+    (ensures fun h0 _ h1 -> modifies (loc o) h0 h1 /\
+      as_nat P384 h1 o = (v c23 * pow2 (3 * 32) + v c23 * pow2 (4 * 32)) % prime384)
+
+let upl_nin_buffer c23 o = 
+  assert_norm (pow2 (1 * 32) * pow2 (2 * 32) = pow2 (3 * 32));
+  assert_norm (pow2 (2 * 32) * pow2 (2 * 32) = pow2 (4 * 32));
+  assert_norm (pow2 (3 * 32) * pow2 (2 * 32) = pow2 (5 * 32));
+  assert_norm (pow2 (4 * 32) * pow2 (2 * 32) = pow2 (6 * 32));
+  assert_norm (pow2 (5 * 32) * pow2 (2 * 32) = pow2 (7 * 32));
+  assert_norm (pow2 (6 * 32) * pow2 (2 * 32) = pow2 (8 * 32));
+  assert_norm (pow2 (7 * 32) * pow2 (2 * 32) = pow2 (9 * 32));
+  assert_norm (pow2 (8 * 32) * pow2 (2 * 32) = pow2 (10 * 32));
+  assert_norm (pow2 (9 * 32) * pow2 (2 * 32) = pow2 (11 * 32));
+
+  let b0 = store_high_low_u (u32 0) (u32 0) in 
+  let b1 = store_high_low_u c23 (u32 0) in 
+  let b2 = store_high_low_u (u32 0) c23 in 
+  let b3 = store_high_low_u (u32 0) (u32 0) in 
+  let b4 = store_high_low_u (u32 0) (u32 0) in 
+  let b5 = store_high_low_u (u32 0) (u32 0) in 
+
+  load_buffer b0 b1 b2 b3 b4 b5 o;
+  reduction_prime_2prime #P384 o o;
+      let h1 = ST.get() in 
+  assert_norm (pow2 (6 * 32) < prime384);
+  modulo_lemma (as_nat P384 h1 o) prime384
+
+
+(* Not sure that FStar will manage to reason about such an input *)
+val solinas_reduction_upload: c0: uint32 -> c1: uint32 ->  c2: uint32 ->  c3: uint32 ->  
+  c4: uint32 ->  c5: uint32 ->  c6: uint32 ->  c7: uint32 ->  c8: uint32 ->  c9: uint32 ->  
+  c10: uint32 ->  c11: uint32 ->  c12: uint32 ->  c13: uint32 ->  c14: uint32 ->  c15: uint32 ->  
+  c16: uint32 ->  c17: uint32 ->  c18: uint32 ->  c19: uint32 ->  c20: uint32 ->  c21: uint32 ->  
+  c22: uint32 ->  c23: uint32 -> 
+  tempBuffer: lbuffer uint64 (size 60) -> 
+  Stack unit 
+    (requires fun h -> live h tempBuffer) 
+    (ensures fun h0 _ h1 -> modifies (loc tempBuffer) h0 h1 /\
+      (
+	let t0 = as_nat P384 h1 (gsub tempBuffer (size 0) (size 6)) in
+        let t1 = as_nat P384 h1 (gsub tempBuffer (size 6) (size 6)) in
+        let t2 = as_nat P384 h1 (gsub tempBuffer (size 12) (size 6)) in
+        let t3 = as_nat P384 h1 (gsub tempBuffer (size 18) (size 6)) in
+        let t4 = as_nat P384 h1 (gsub tempBuffer (size 24) (size 6)) in
+        let t5 = as_nat P384 h1 (gsub tempBuffer (size 30) (size 6)) in
+        let t6 = as_nat P384 h1 (gsub tempBuffer (size 36) (size 6)) in
+        let t7 = as_nat P384 h1 (gsub tempBuffer (size 42) (size 6)) in
+        let t8 = as_nat P384 h1 (gsub tempBuffer (size 48) (size 6)) in
+	let t9 = as_nat P384 h1 (gsub tempBuffer (size 54) (size 6)) in 
+	t0 = (v c0 + v c1 * pow2 (1 * 32) + v c2 * pow2 (2 * 32) + v c3 * pow2 (3 * 32) + v c4 * pow2 (4 * 32) + v c5 * pow2 (5 * 32) + v c6 * pow2 (6 * 32) + v c7 * pow2 (7 * 32) + v c8 * pow2 (8 * 32) + v c9 * pow2 (9 * 32) + v c10 * pow2 (10 * 32) + v c11 * pow2 (11 * 32)) % prime384 /\
+	t1 = (v c21 * pow2 (4 * 32) + v c22 * pow2 (5 * 32) + v c23 * pow2 (6 * 32)) % prime384 /\
+	t2 = (v c12 + v c13 * pow2 (1 * 32) + v c14 * pow2 (2 * 32) + v c15 * pow2 (3 * 32) + v c16 * pow2 (4 * 32) + v c17 * pow2 (5 * 32) + v c18 * pow2 (6 * 32) + v c19 * pow2 (7 * 32) + v c20 * pow2 (8 * 32) + v c21 * pow2 (9 * 32) + v c22 * pow2 (10 * 32) + v c23 * pow2 (11 * 32)) % prime384 /\
+	t3 = (v c21 + v c22 * pow2 (1 * 32) + v c23 * pow2 (2 * 32) + v c12 * pow2 (3 * 32) + v c13 * pow2 (4 * 32) + v c14 * pow2 (5 * 32) + v c15 * pow2 (6 * 32) + v c16 * pow2 (7 * 32) + v c17 * pow2 (8 * 32) + v c18 * pow2 (9 * 32) + v c19 * pow2 (10 * 32) + v c20 * pow2 (11 * 32)) % prime384 /\
+	t4 = (v c23 * pow2 (1 * 32) + v c20 * pow2 (3 * 32) + v c12 * pow2 (4 * 32) + v c13 * pow2 (5 * 32) + v c14 * pow2 (6 * 32) + v c15 * pow2 (7 * 32) + v c16 * pow2 (8 * 32) + v c17 * pow2 (9 * 32) + v c18 * pow2 (10 * 32) + v c19 * pow2 (11 * 32)) % prime384 /\
+	t5 = (v c20 * pow2 (4 * 32) + v c21 * pow2 (5 * 32) + v c22 * pow2 (6 * 32) + v c23 * pow2 (7 * 32)) % prime384 /\
+	t6 = (v c20 + v c21 * pow2 (3 * 32) + v c22 * pow2 (4 * 32) + v c23 * pow2 (5 * 32)) % prime384 /\
+	t7 = (v c23 + v c12 * pow2 (1 * 32) + v c13 * pow2 (2 * 32) + v c14 * pow2 (3 * 32) + v c15 * pow2 (4 * 32) + v c16 * pow2 (5 * 32) + v c17 * pow2 (6 * 32) + v c18 * pow2 (7 * 32) + v c19 * pow2 (8 * 32) + v c20 * pow2 (9 * 32) + v c21 * pow2 (10 * 32) + v c22 * pow2 (11 * 32)) % prime384 /\
+	t8 = (v c20 * pow2 (1 * 32) + v c21 * pow2 (2 * 32) + v c22 * pow2 (3 * 32) + v c23 * pow2 (4 * 32)) % prime384 /\
+	t9 = (v c23 * pow2 (3 * 32) + v c23 * pow2 (4 * 32)) % prime384
+      )
+  )
+    
+
+let solinas_reduction_upload c0 c1 c2 c3 c4 c5 c6 c7 c8 c9 c10 c11 c12 c13 c14 c15 c16 c17 c18 c19 c20 c21 c22 c23 tempBuffer = 
+  let t0 = sub tempBuffer (size 0) (size 6) in 
+  let t1 = sub tempBuffer (size 6) (size 6) in 
+  let t2 = sub tempBuffer (size 12) (size 6) in 
+  let t3 = sub tempBuffer (size 18) (size 6) in 
+  let t4 = sub tempBuffer (size 24) (size 6) in 
+  let t5 = sub tempBuffer (size 30) (size 6) in 
+  let t6 = sub tempBuffer (size 36) (size 6) in 
+  let t7 = sub tempBuffer (size 42) (size 6) in 
+  let t8 = sub tempBuffer (size 48) (size 6) in 
+  let t9 = sub tempBuffer (size 54) (size 6) in 
+    
+  upl_zer_buffer c0 c1 c2 c3 c4 c5 c6 c7 c8 c9 c10 c11 t0;
+  upl_fir_buffer c21 c22 c23 t1;
+  upl_sec_buffer c12 c13 c14 c15 c16 c17 c18 c19 c20 c21 c22 c23 t2;
+  upl_thi_buffer c12 c13 c14 c15 c16 c17 c18 c19 c20 c21 c22 c23 t3;
+  upl_forth_buffer c12 c13 c14 c15 c16 c17 c18 c19 c20 c23 t4;
+  upl_fif_buffer c20 c21 c22 c23 t5;
+  upl_six_buffer c20 c21 c22 c23 t6;
+  upl_sev_buffer c12 c13 c14 c15 c16 c17 c18 c19 c20 c21 c22 c23 t7;
+  upl_eit_buffer c20 c21 c22 c23 t8;
+  upl_nin_buffer c23 t9
+
+
+val solinas_reduction_operations: tempBuffer: lbuffer uint64 (size 60) -> o: lbuffer uint64 (size 6) -> 
+  Stack unit 
+    (requires fun h -> live h o /\ live h tempBuffer /\ disjoint tempBuffer o /\
+      (
+          let t0 = as_nat P384 h (gsub tempBuffer (size 0) (size 6)) in
+          let t1 = as_nat P384 h (gsub tempBuffer (size 6) (size 6)) in
+          let t2 = as_nat P384 h (gsub tempBuffer (size 12) (size 6)) in
+          let t3 = as_nat P384 h (gsub tempBuffer (size 18) (size 6)) in
+          let t4 = as_nat P384 h (gsub tempBuffer (size 24) (size 6)) in
+          let t5 = as_nat P384 h (gsub tempBuffer (size 30) (size 6)) in
+          let t6 = as_nat P384 h (gsub tempBuffer (size 36) (size 6)) in
+          let t7 = as_nat P384 h (gsub tempBuffer (size 42) (size 6)) in
+          let t8 = as_nat P384 h (gsub tempBuffer (size 48) (size 6)) in
+	  let t9 = as_nat P384 h (gsub tempBuffer (size 54) (size 6)) in 
+          t0 < prime384 /\ t1 < prime384 /\ t2 < prime384 /\ t3 < prime384 /\ t4 < prime384 /\
+          t5 < prime384 /\ t6 < prime384 /\ t7 < prime384 /\ t8 < prime384 /\ t9 < prime384
+      ) 
+    )
+    (ensures fun h0 _ h1 -> modifies (loc tempBuffer |+| loc o) h0 h1 /\
+      (
+	let t0 = as_nat P384 h0 (gsub tempBuffer (size 0) (size 6)) in
+        let t1 = as_nat P384 h0 (gsub tempBuffer (size 6) (size 6)) in
+        let t2 = as_nat P384 h0 (gsub tempBuffer (size 12) (size 6)) in
+        let t3 = as_nat P384 h0 (gsub tempBuffer (size 18) (size 6)) in
+        let t4 = as_nat P384 h0 (gsub tempBuffer (size 24) (size 6)) in
+        let t5 = as_nat P384 h0 (gsub tempBuffer (size 30) (size 6)) in
+        let t6 = as_nat P384 h0 (gsub tempBuffer (size 36) (size 6)) in
+        let t7 = as_nat P384 h0 (gsub tempBuffer (size 42) (size 6)) in
+        let t8 = as_nat P384 h0 (gsub tempBuffer (size 48) (size 6)) in
+	let t9 = as_nat P384 h0 (gsub tempBuffer (size 54) (size 6)) in 
+	as_nat P384 h1 o = (t0 + 2 * t1 + t2 + t3 + t4 + t5 + t6 - t7 - t8 - t9) % prime384
+      )
+    )
+    
+
+let solinas_reduction_operations tempBuffer o = 
+  let t0 = sub tempBuffer (size 0) (size 6) in
+  let t1 = sub tempBuffer (size 6) (size 6) in
+  let t2 = sub tempBuffer (size 12) (size 6) in
+  let t3 = sub tempBuffer (size 18) (size 6) in
+  let t4 = sub tempBuffer (size 24) (size 6) in
+  let t5 = sub tempBuffer (size 30) (size 6) in
+  let t6 = sub tempBuffer (size 36) (size 6) in
+  let t7 = sub tempBuffer (size 42) (size 6) in
+  let t8 = sub tempBuffer (size 48) (size 6) in
+  let t9 = sub tempBuffer (size 54) (size 6) in 
+
+  let h0 = ST.get() in 
+
+  felem_double #P384 t1 t1;
+  felem_add #P384 t0 t1 t1;
+  felem_add #P384 t1 t2 t2;
+  felem_add #P384 t2 t3 t3;
+  felem_add #P384 t3 t4 t4;
+  felem_add #P384 t4 t5 t5;
+  felem_add #P384 t5 t6 t6;
+  felem_sub #P384 t6 t7 t7;
+  felem_sub #P384 t7 t8 t8;
+  felem_sub #P384 t8 t9 o;
+
+  let h1 = ST.get() in 
+  assert(as_nat P384 h1 o = ((((((((((as_nat P384 h1 t0 + (as_nat P384 h0 t1 + as_nat P384 h0 t1) % prime384) % prime384 + as_nat P384 h0 t2) % prime384) + as_nat P384 h0 t3) % prime384 + as_nat P384 h0 t4) % prime384 + as_nat P384 h0 t5) % prime384 + as_nat P384 h0 t6) % prime384 - as_nat P384 h0 t7) % prime384 - as_nat P384 h0 t8) % prime384 - as_nat P384 h0 t9) % prime384);
+
+  calc (==) {
+  as_nat P384 h1 o;
+  (==) {}
+  ((((((((((as_nat P384 h1 t0 + (as_nat P384 h0 t1 + as_nat P384 h0 t1) % prime384) % prime384 + as_nat P384 h0 t2) % prime384) + as_nat P384 h0 t3) % prime384 + as_nat P384 h0 t4) % prime384 + as_nat P384 h0 t5) % prime384 + as_nat P384 h0 t6) % prime384 - as_nat P384 h0 t7) % prime384 - as_nat P384 h0 t8) % prime384 - as_nat P384 h0 t9) % prime384;
+  (==)
+  {lemma_mod_add_distr (as_nat P384 h1 t0) (as_nat P384 h0 t1 + as_nat P384 h0 t1) prime384}
+  ((((((((((as_nat P384 h1 t0 + as_nat P384 h0 t1 + as_nat P384 h0 t1) % prime384 + as_nat P384 h0 t2) % prime384) + as_nat P384 h0 t3) % prime384 + as_nat P384 h0 t4) % prime384 + as_nat P384 h0 t5) % prime384 + as_nat P384 h0 t6) % prime384 - as_nat P384 h0 t7) % prime384 - as_nat P384 h0 t8) % prime384 - as_nat P384 h0 t9) % prime384;
+  (==) 
+  {lemma_mod_add_distr (as_nat P384 h0 t2) (as_nat P384 h1 t0 + as_nat P384 h0 t1 + as_nat P384 h0 t1) prime384}
+  (((((((((as_nat P384 h1 t0 + as_nat P384 h0 t1 + as_nat P384 h0 t1 + as_nat P384 h0 t2) % prime384) + as_nat P384 h0 t3) % prime384 + as_nat P384 h0 t4) % prime384 + as_nat P384 h0 t5) % prime384 + as_nat P384 h0 t6) % prime384 - as_nat P384 h0 t7) % prime384 - as_nat P384 h0 t8) % prime384 - as_nat P384 h0 t9) % prime384;
+  (==)
+  {lemma_mod_add_distr (as_nat P384 h0 t3) (as_nat P384 h1 t0 + as_nat P384 h0 t1 + as_nat P384 h0 t1 + as_nat P384 h0 t2) prime384}
+  (((((((as_nat P384 h1 t0 + as_nat P384 h0 t1 + as_nat P384 h0 t1 + as_nat P384 h0 t2 + as_nat P384 h0 t3) % prime384 + as_nat P384 h0 t4) % prime384 + as_nat P384 h0 t5) % prime384 + as_nat P384 h0 t6) % prime384 - as_nat P384 h0 t7) % prime384 - as_nat P384 h0 t8) % prime384 - as_nat P384 h0 t9) % prime384;
+  (==)
+  {lemma_mod_add_distr (as_nat P384 h0 t4) (as_nat P384 h1 t0 + as_nat P384 h0 t1 + as_nat P384 h0 t1 + as_nat P384 h0 t2 + as_nat P384 h0 t3) prime384}
+  ((((((as_nat P384 h1 t0 + as_nat P384 h0 t1 + as_nat P384 h0 t1 + as_nat P384 h0 t2 + as_nat P384 h0 t3 + as_nat P384 h0 t4) % prime384 + as_nat P384 h0 t5) % prime384 + as_nat P384 h0 t6) % prime384 - as_nat P384 h0 t7) % prime384 - as_nat P384 h0 t8) % prime384 - as_nat P384 h0 t9) % prime384;
+  (==) 
+  {lemma_mod_add_distr (as_nat P384 h0 t5) (as_nat P384 h1 t0 + as_nat P384 h0 t1 + as_nat P384 h0 t1 + as_nat P384 h0 t2 + as_nat P384 h0 t3 + as_nat P384 h0 t4) prime384}
+  (((((as_nat P384 h1 t0 + as_nat P384 h0 t1 + as_nat P384 h0 t1 + as_nat P384 h0 t2 + as_nat P384 h0 t3 + as_nat P384 h0 t4 + as_nat P384 h0 t5) % prime384 + as_nat P384 h0 t6) % prime384 - as_nat P384 h0 t7) % prime384 - as_nat P384 h0 t8) % prime384 - as_nat P384 h0 t9) % prime384;
+  (==) 
+  {lemma_mod_add_distr (as_nat P384 h0 t6) (as_nat P384 h1 t0 + as_nat P384 h0 t1 + as_nat P384 h0 t1 + as_nat P384 h0 t2 + as_nat P384 h0 t3 + as_nat P384 h0 t4 + as_nat P384 h0 t5) prime384}
+  ((((as_nat P384 h1 t0 + as_nat P384 h0 t1 + as_nat P384 h0 t1 + as_nat P384 h0 t2 + as_nat P384 h0 t3 + as_nat P384 h0 t4 + as_nat P384 h0 t5 + as_nat P384 h0 t6) % prime384 - as_nat P384 h0 t7) % prime384 - as_nat P384 h0 t8) % prime384 - as_nat P384 h0 t9) % prime384;
+  (==)
+  {lemma_mod_add_distr (-as_nat P384 h0 t7) (as_nat P384 h1 t0 + as_nat P384 h0 t1 + as_nat P384 h0 t1 + as_nat P384 h0 t2 + as_nat P384 h0 t3 + as_nat P384 h0 t4 + as_nat P384 h0 t5 + as_nat P384 h0 t6) prime384}
+  (((as_nat P384 h1 t0 + as_nat P384 h0 t1 + as_nat P384 h0 t1 + as_nat P384 h0 t2 + as_nat P384 h0 t3 + as_nat P384 h0 t4 + as_nat P384 h0 t5 + as_nat P384 h0 t6 - as_nat P384 h0 t7) % prime384 - as_nat P384 h0 t8) % prime384 - as_nat P384 h0 t9) % prime384;
+  (==)
+  {lemma_mod_add_distr (- as_nat P384 h0 t8) (as_nat P384 h1 t0 + as_nat P384 h0 t1 + as_nat P384 h0 t1 + as_nat P384 h0 t2 + as_nat P384 h0 t3 + as_nat P384 h0 t4 + as_nat P384 h0 t5 + as_nat P384 h0 t6 - as_nat P384 h0 t7) prime384}
+  ((as_nat P384 h1 t0 + as_nat P384 h0 t1 + as_nat P384 h0 t1 + as_nat P384 h0 t2 + as_nat P384 h0 t3 + as_nat P384 h0 t4 + as_nat P384 h0 t5 + as_nat P384 h0 t6 - as_nat P384 h0 t7 - as_nat P384 h0 t8) % prime384 - as_nat P384 h0 t9) % prime384;
+  (==)
+  {lemma_mod_add_distr (- as_nat P384 h0 t9) (as_nat P384 h1 t0 + as_nat P384 h0 t1 + as_nat P384 h0 t1 + as_nat P384 h0 t2 + as_nat P384 h0 t3 + as_nat P384 h0 t4 + as_nat P384 h0 t5 + as_nat P384 h0 t6 - as_nat P384 h0 t7 - as_nat P384 h0 t8) prime384}
+  (as_nat P384 h1 t0 + 2 * as_nat P384 h0 t1 + as_nat P384 h0 t2 + as_nat P384 h0 t3 + as_nat P384 h0 t4 + as_nat P384 h0 t5 + as_nat P384 h0 t6 - as_nat P384 h0 t7 - as_nat P384 h0 t8 - as_nat P384 h0 t9) % prime384;}
+
+
+let _uint32 = n:nat{n < pow2 32}
+
+assume val solinas_reduction_mod:
+  c0_n: _uint32->
+  c1_n: _uint32 ->
+  c2_n: _uint32 ->
+  c3_n: _uint32 ->
+  c4_n: _uint32 ->
+  c5_n: _uint32 ->
+  c6_n: _uint32 ->
+  c7_n: _uint32 ->
+  c8_n: _uint32 ->
+  c9_n: _uint32 ->
+  c10_n: _uint32 ->
+  c11_n: _uint32 ->
+  c12_n: _uint32 ->
+  c13_n: _uint32 ->
+  c14_n: _uint32 ->
+  c15_n: _uint32 ->
+  c16_n: _uint32 -> 
+  c17_n: _uint32 -> 
+  c18_n: _uint32 -> 
+  c19_n: _uint32 -> 
+  c20_n: _uint32 -> 
+  c21_n: _uint32 -> 
+  c22_n: _uint32 -> 
+  c23_n: _uint32 ->
+  s0: nat {s0 = (c0_n + c1_n * pow2 (1 * 32) + c2_n * pow2 (2 * 32) + c3_n * pow2 (3 * 32) + c4_n * pow2 (4 * 32) + c5_n * pow2 (5 * 32) + c6_n * pow2 (6 * 32) + c7_n * pow2 (7 * 32) + c8_n * pow2 (8 * 32) + c9_n * pow2 (9 * 32) + c10_n * pow2 (10 * 32) + c11_n * pow2 (11 * 32)) % prime384} ->
+  s1: nat {s1 = (c21_n * pow2 (4 * 32) + c22_n * pow2 (5 * 32) + c23_n * pow2 (6 * 32)) % prime384} ->
+  s2: nat {s2 = (c12_n + c13_n * pow2 (1 * 32) + c14_n * pow2 (2 * 32) + c15_n * pow2 (3 * 32) + c16_n * pow2 (4 * 32) + c17_n * pow2 (5 * 32) + c18_n * pow2 (6 * 32) + c19_n * pow2 (7 * 32) + c20_n * pow2 (8 * 32) + c21_n * pow2 (9 * 32) + c22_n * pow2 (10 * 32) + c23_n * pow2 (11 * 32)) % prime384} ->
+  s3: nat {s3 = (c21_n + c22_n * pow2 (1 * 32) + c23_n * pow2 (2 * 32) + c12_n * pow2 (3 * 32) + c13_n * pow2 (4 * 32) + c14_n * pow2 (5 * 32) + c15_n * pow2 (6 * 32) + c16_n * pow2 (7 * 32) + c17_n * pow2 (8 * 32) + c18_n * pow2 (9 * 32) + c19_n * pow2 (10 * 32) + c20_n * pow2 (11 * 32)) % prime384} ->
+  s4: nat {s4 = (c23_n * pow2 (1 * 32) + c20_n * pow2 (3 * 32) + c12_n * pow2 (4 * 32) + c13_n * pow2 (5 * 32) + c14_n * pow2 (6 * 32) + c15_n * pow2 (7 * 32) + c16_n * pow2 (8 * 32) + c17_n * pow2 (9 * 32) + c18_n * pow2 (10 * 32) + c19_n * pow2 (11 * 32)) % prime384} ->
+  s5: nat {s5 = (c20_n * pow2 (4 * 32) + c21_n * pow2 (5 * 32) + c22_n * pow2 (6 * 32) + c23_n * pow2 (7 * 32)) % prime384} ->
+  s6: nat {s6 = (c20_n + c21_n * pow2 (3 * 32) + c22_n * pow2 (4 * 32) + c23_n * pow2 (5 * 32)) % prime384} ->
+  s7: nat {s7 = (c23_n + c12_n * pow2 (1 * 32) + c13_n * pow2 (2 * 32) + c14_n * pow2 (3 * 32) + c15_n * pow2 (4 * 32) + c16_n * pow2 (5 * 32) + c17_n * pow2 (6 * 32) + c18_n * pow2 (7 * 32) + c19_n * pow2 (8 * 32) + c20_n * pow2 (9 * 32) + c21_n * pow2 (10 * 32) + c22_n * pow2 (11 * 32)) % prime384} ->
+  s8: nat {s8 = (c20_n * pow2 (1 * 32) + c21_n * pow2 (2 * 32) + c22_n * pow2 (3 * 32) + c23_n * pow2 (4 * 32)) % prime384} ->
+  s9: nat {s9 = (c23_n * pow2 (3 * 32) + c23_n * pow2 (4 * 32)) % prime384} ->
+  n: int {n = (s0 + 2 * s1 + s2 + s3 + s4 + s5 + s6 - s7 - s8 - s9) % prime384} ->
+  Lemma (n % prime384 == (c0_n + c1_n * pow2 32 + c2_n * pow2 (2 * 32) + c3_n * pow2 (3 * 32) + c4_n * pow2 (4 * 32) + c5_n * pow2 (5 * 32) + c6_n * pow2 (6 * 32) + c7_n * pow2 (7 * 32) + c8_n * pow2 256 + c9_n * pow2 (9 * 32) + c10_n * pow2 (10 * 32)  + c11_n * pow2 (11 * 32) + c12_n * pow2 (12 * 32) + c13_n* pow2 (13 * 32) + c14_n * pow2 (14 * 32) + c15_n * pow2 (15 * 32) + c16_n * pow2 (16 * 32) + c17_n * pow2 (17 * 32) + c18_n * pow2 (18 * 32) + c19_n * pow2 (19 * 32) + c20_n * pow2 (20 * 32) + c21_n * pow2 (21 * 32) + c22_n * pow2 (22 * 32) + c23_n * pow2 (23 * 32)) % prime384)
+
+
+
+assume val lemma_opened: i:Lib.Sequence.lseq uint64 12 -> Lemma
+  (let open Lib.Sequence in
+   
+    let i0 = index i 0 in
+    let i1 = index i 1 in
+    let i2 = index i 2 in
+    let i3 = index i 3 in
+    let i4 = index i 4 in
+    let i5 = index i 5 in
+    let i6 = index i 6 in
+    let i7 = index i 7 in
+    let i8 = index i 8 in 
+    let i9 = index i 9 in 
+    let i10 = index i 10 in 
+    let i11 = index i 11 in 
+
+
+    let c0 = get_low_part i0 in
+    let c1 = get_high_part i0 in
+    let c2 = get_low_part i1 in
+    let c3 = get_high_part i1 in
+    let c4 = get_low_part i2 in
+    let c5 = get_high_part i2 in
+    let c6 = get_low_part i3 in
+    let c7 = get_high_part i3 in
+    let c8 = get_low_part i4 in
+    let c9 = get_high_part i4 in
+    let c10 = get_low_part i5 in
+    let c11 = get_high_part i5 in
+    let c12 = get_low_part i6 in
+    let c13 = get_high_part i6 in
+    let c14 = get_low_part i7 in
+    let c15 = get_high_part i7 in
+    let c16 = get_low_part i8 in 
+    let c17 = get_high_part i8 in 
+    let c18 = get_low_part i9 in 
+    let c19 = get_high_part i9 in 
+    let c20 = get_low_part i10 in 
+    let c21 = get_high_part i10 in 
+    let c22 = get_low_part i11 in 
+    let c23 = get_high_part i11 in 
+
+    felem_seq_as_nat_16 i = 
+     v c0  * pow2 (0 * 32) +
+     v c1  * pow2 (1 * 32) +
+     v c2  * pow2 (2 * 32) +
+     v c3  * pow2 (3 * 32) +
+     v c4  * pow2 (4 * 32) +
+     v c5  * pow2 (5 * 32) +
+     v c6  * pow2 (6 * 32) +
+     v c7  * pow2 (7 * 32) +
+     v c8  * pow2 (8 * 32) +
+     v c9  * pow2 (9 * 32) +
+     v c10 * pow2 (10 * 32) +
+     v c11 * pow2 (11 * 32) +
+     v c12 * pow2 (12 * 32) +
+     v c13 * pow2 (13 * 32) +
+     v c14 * pow2 (14 * 32) +
+     v c15 * pow2 (15 * 32) + 
+     v c16 * pow2 (16 * 32) + 
+     v c17 * pow2 (17 * 32) + 
+     v c18 * pow2 (18 * 32) + 
+     v c19 * pow2 (19 * 32) + 
+     v c20 * pow2 (20 * 32) + 
+     v c21 * pow2 (21 * 32) +
+     v c22 * pow2 (22 * 32) + 
+     v c23 * pow2 (23 * 32)
+  ) 
+
+
+
+let solinasReduction384Impl i o = 
+  push_frame();
+    let h0 = ST.get() in
+    let tempBuffer = create (size 60) (u64 0) in
+
+    let t0 = sub tempBuffer (size 0) (size 6) in 
+    let t1 = sub tempBuffer (size 6) (size 6) in 
+    let t2 = sub tempBuffer (size 12) (size 6) in 
+    let t3 = sub tempBuffer (size 18) (size 6) in 
+    let t4 = sub tempBuffer (size 24) (size 6) in 
+    let t5 = sub tempBuffer (size 30) (size 6) in 
+    let t6 = sub tempBuffer (size 36) (size 6) in 
+    let t7 = sub tempBuffer (size 42) (size 6) in 
+    let t8 = sub tempBuffer (size 48) (size 6) in 
+    let t9 = sub tempBuffer (size 54) (size 6) in 
+    
+    let i0 = i.(size 0) in
+    let i1 = i.(size 1) in
+    let i2 = i.(size 2) in
+    let i3 = i.(size 3) in
+    let i4 = i.(size 4) in
+    let i5 = i.(size 5) in
+    let i6 = i.(size 6) in
+    let i7 = i.(size 7) in
+    let i8 = i.(size 8) in 
+    let i9 = i.(size 9) in 
+    let i10 = i.(size 10) in 
+    let i11 = i.(size 11) in 
+  
+    let c0 = get_low_part i0 in
+    let c1 = get_high_part i0 in
+    let c2 = get_low_part i1 in
+    let c3 = get_high_part i1 in
+    let c4 = get_low_part i2 in
+    let c5 = get_high_part i2 in
+    let c6 = get_low_part i3 in
+    let c7 = get_high_part i3 in
+    let c8 = get_low_part i4 in
+    let c9 = get_high_part i4 in
+    let c10 = get_low_part i5 in
+    let c11 = get_high_part i5 in
+    let c12 = get_low_part i6 in
+    let c13 = get_high_part i6 in
+    let c14 = get_low_part i7 in
+    let c15 = get_high_part i7 in
+    let c16 = get_low_part i8 in 
+    let c17 = get_high_part i8 in 
+    let c18 = get_low_part i9 in 
+    let c19 = get_high_part i9 in 
+    let c20 = get_low_part i10 in 
+    let c21 = get_high_part i10 in 
+    let c22 = get_low_part i11 in 
+    let c23 = get_high_part i11 in 
+
+    solinas_reduction_upload c0 c1 c2 c3 c4 c5 c6 c7 c8 c9 c10 c11 c12 c13 c14 c15 c16 c17 c18 c19 c20 c21 c22 c23 tempBuffer;
+      let h1 = ST.get() in 
+    solinas_reduction_operations tempBuffer o;
+      let h2 = ST.get() in  
+    solinas_reduction_mod (v c0) (v c1) (v c2) (v c3) (v c4) (v c5) (v c6) (v c7) (v c8) (v c9) (v c10) (v c11) (v c12) (v c13) (v c14) (v c15) (v c16) (v c17) (v c18) (v c19) (v c20) (v c21) (v c22) (v c23)
+    (as_nat P384 h1 t0) (as_nat P384 h1 t1) (as_nat P384 h1 t2) (as_nat P384 h1 t3) (as_nat P384 h1 t4) (as_nat P384 h1 t5) (as_nat P384 h1 t6) (as_nat P384 h1 t7) (as_nat P384 h1 t8) (as_nat P384 h1 t9) (as_nat P384 h2 o); 
+    modulo_lemma (as_nat P384 h2 o) prime384;
+    lemma_opened (as_seq h0 i);
+    pop_frame()
