code/ecdsap256/Hacl.Impl.SolinasReduction.P384.fsti
@@ -1,0 +1,22 @@
+module Hacl.Impl.SolinasReduction.P384
+
+
+open FStar.HyperStack.All
+open FStar.HyperStack
+
+module ST = FStar.HyperStack.ST
+
+open FStar.Math
+open FStar.Math.Lemmas
+open FStar.Mul
+
+open Lib.IntTypes
+open Lib.Buffer
+
+open Spec.P256
+open Hacl.Spec.P256.Definition
+
+val solinasReduction384Impl: i: lbuffer uint64 (size 12) -> o: lbuffer uint64 (size 6) -> 
+  Stack unit 
+    (requires fun h -> live h i /\ live h o /\ disjoint i o)
+    (ensures fun h0 _ h1 -> modifies (loc o) h0 h1 /\ wide_as_nat P384 h0 i % prime384 = as_nat P384 h1 o)
